src/Tom_proof.thy
@@ -16,4 +16,36 @@ wellformed_ts ts'
 ))
 "
 
+lemma invariant_wf_ts: "invariant_wf_ts"
+apply(simp add: invariant_wf_ts_def)
+apply(intro allI impI)
+apply(case_tac ts)
+apply(case_tac x)
+apply(rename_tac f stk)
+apply(simp add: step_tree_stack_def dest_ts_def)
+apply(case_tac stk) apply(force)
+apply(rename_tac ni stk)
+apply(case_tac ni)
+apply(rename_tac n i)
+apply(simp)
+apply(thin_tac "ts = _")
+apply(thin_tac "x = _")
+apply(thin_tac "stka = _")
+apply(thin_tac "ni = _")
+apply(simp add: wellformed_ts_def)
+apply(simp add: dest_ts_def)
+apply(elim conjE)
+apply(intro conjI)
+ (* wf_focus *)
+ apply(simp add: wellformed_focus_def )
+ apply()
+
+ (* wf_context *)
+
+
+  (* wf_ts_1 *)
+
+end
+
+
 end
